casestudies/compcert/lib/Prelude.v
@@ -3,6 +3,9 @@ Require Import Mergesort.
 Require Import Ordered.
 From NFPOP Require Import Coqlib.
 From NFPOP Require Import AST.
+From NFPOP Require Import Maps.
+From NFPOP Require Import Values.
+From NFPOP Require Import Integers. 
 Require Import Coq.ZArith.ZArith.
 
 Axiom cheat : forall {X}, X.
@@ -19,3 +22,84 @@ Module VarOrder <: TotalLeBool.
 End VarOrder.
 
 Module VarSort := Mergesort.Sort(VarOrder).
+
+
+(* Registers for Asm *)
+
+Inductive ireg: Type :=
+  | X1:  ireg | X2:  ireg | X3:  ireg | X4:  ireg | X5:  ireg
+  | X6:  ireg | X7:  ireg | X8:  ireg | X9:  ireg | X10: ireg
+  | X11: ireg | X12: ireg | X13: ireg | X14: ireg | X15: ireg
+  | X16: ireg | X17: ireg | X18: ireg | X19: ireg | X20: ireg
+  | X21: ireg | X22: ireg | X23: ireg | X24: ireg | X25: ireg
+  | X26: ireg | X27: ireg | X28: ireg | X29: ireg | X30: ireg
+  | X31: ireg.
+
+Inductive ireg0: Type :=
+  | X0: ireg0 | X: ireg -> ireg0.
+
+Coercion X: ireg >-> ireg0.
+
+(** Floating-point registers *)
+
+Inductive freg: Type :=
+  | F0: freg  | F1: freg  | F2: freg  | F3: freg
+  | F4: freg  | F5: freg  | F6: freg  | F7: freg
+  | F8: freg  | F9: freg  | F10: freg | F11: freg
+  | F12: freg | F13: freg | F14: freg | F15: freg
+  | F16: freg | F17: freg | F18: freg | F19: freg
+  | F20: freg | F21: freg | F22: freg | F23: freg
+  | F24: freg | F25: freg | F26: freg | F27: freg
+  | F28: freg | F29: freg | F30: freg | F31: freg.
+
+Lemma ireg_eq: forall (x y: ireg), {x=y} + {x<>y}.
+Proof. decide equality. Defined.
+
+Lemma ireg0_eq: forall (x y: ireg0), {x=y} + {x<>y}.
+Proof. decide equality. apply ireg_eq. Defined.
+
+Lemma freg_eq: forall (x y: freg), {x=y} + {x<>y}.
+Proof. decide equality. Defined.
+  
+(** We model the following registers of the RISC-V architecture. *)
+
+Inductive preg: Type :=
+  | IR: ireg -> preg                    (**r integer registers *)
+  | FR: freg -> preg                    (**r double-precision float registers *)
+  | PC: preg.                           (**r program counter *)
+
+Coercion IR: ireg >-> preg.
+Coercion FR: freg >-> preg.
+
+Lemma preg_eq: forall (x y: preg), {x=y} + {x<>y}.
+Proof. decide equality. apply ireg_eq. apply freg_eq. Defined.
+
+Module PregEq.
+  Definition t  := preg.
+  Definition eq := preg_eq.
+End PregEq.
+
+Module Pregmap := EMap(PregEq).
+
+(** Conventional names for stack pointer ([SP]) and return address ([RA]). *)
+
+Declare Scope asm.
+Notation "'SP'" := X2 (only parsing) : asm.
+Notation "'RA'" := X1 (only parsing) : asm.
+
+Definition get0w (rs: Pregmap.t val) (r: ireg0) : val :=
+  match r with
+  | X0 => Vint Int.zero
+  | X r => rs r
+  end.
+
+Definition get0l (rs: Pregmap.t val) (r: ireg0) : val :=
+  match r with
+  | X0 => Vlong Int64.zero
+  | X r => rs r
+  end.
+
+Notation "a # b" := (a b) (at level 1, only parsing) : asm.
+Notation "a ## b" := (get0w a b) (at level 1) : asm.
+Notation "a ### b" := (get0l a b) (at level 1) : asm.
+Notation "a # b <- c" := (Pregmap.set b c a) (at level 1, b at next level) : asm.
